

Recurrences

Shirley B. Chu

De La Salle University

10 Apr 2023



Recurrence

- **Recurrence** is used to describe the running time of a recursive algorithm.

Recurrence

- **Recurrence** is used to describe the running time of a recursive algorithm.

Iterative, not recursive

```
int factorial (int n)
{
    int result = 1;
    while (n > 0)
    {
        result *= n;
        n--;
    }
    return result;
}
```

Recurrence

- **Recurrence** is used to describe the running time of a recursive algorithm.

Iterative, not recursive

```
int factorial (int n)
{
    int result = 1;
    while (n > 0)
    {
        result *= n;
        n--;
    }
    return result;
}
```

Recursive

```
int factorial (int n)
{
    if (n == 0)
        return 1;

    return n * factorial (n - 1);
}
```

Recurrence

- **Recurrence** is used to describe the running time of a recursive algorithm.

Iterative, not recursive

```
int factorial (int n)
{
    int result = 1;
    while (n > 0)
    {
        result *= n;
        n--;
    }
    return result;
}
```

Recursive

```
int factorial (int n)
{
    if (n == 0)
        return 1;

    return n * factorial (n - 1);
}
```

- A general form of recurrence is an equality or inequality that describes a function over integers or reals using the function itself.

Recurrence

- **Recurrence** is used to describe the running time of a recursive algorithm.

Iterative, not recursive

```
int factorial (int n)
{
    int result = 1;
    while (n > 0)
    {
        result *= n;
        n--;
    }
    return result;
}
```

Recursive

```
int factorial (int n)
{
    if (n == 0)
        return 1;

    return n * factorial (n - 1);
}
```

- A general form of recurrence is an equality or inequality that describes a function over integers or reals using the function itself.
- It contains **more than one** cases, depending on the argument.

Recurrence

- **Recurrence** is used to describe the running time of a recursive algorithm.

Iterative, not recursive

```
int factorial (int n)
{
    int result = 1;
    while (n > 0)
    {
        result *= n;
        n--;
    }
    return result;
}
```

Recursive

```
int factorial (int n)
{
    if (n == 0)
        return 1;

    return n * factorial (n - 1);
}
```

- A general form of recurrence is an equality or inequality that describes a function over integers or reals using the function itself.
- It contains **more than one** cases, depending on the argument.
 - **recursive case**

Recurrence

- **Recurrence** is used to describe the running time of a recursive algorithm.

Iterative, not recursive

```
int factorial (int n)
{
    int result = 1;
    while (n > 0)
    {
        result *= n;
        n--;
    }
    return result;
}
```

Recursive

```
int factorial (int n)
{
    if (n == 0)
        return 1;

    return n * factorial (n - 1);
}
```

- A general form of recurrence is an equality or inequality that describes a function over integers or reals using the function itself.
- It contains **more than one** cases, depending on the argument.
 - **recursive case**
 - **base case**

Example 1: factorial()

```
int factorial (int n)
{
    if (n == 0)
        return 1;

    return n * factorial (n - 1);
}
```

Example 1: factorial()

```
int factorial (int n)
{
    if (n == 0)
        return 1;

    return n * factorial (n - 1);
}
```

$$T(n) =$$

Example 1: factorial()

```
int factorial (int n)
```

```
{
```

```
    if (n == 0)
```

```
        return 1;
```

```
    return n * factorial (n - 1);
```

```
}
```

$$T(n) = \left\{ \right.$$

Example 1: factorial()

```
int factorial (int n)
{
    if (n == 0)
        return 1;

    return n * factorial (n - 1);
}
```

$$T(n) = \begin{cases} n == 0 \end{cases}$$

Example 1: factorial()

```
int factorial (int n)
{
    if (n == 0)
        return 1;

    return n * factorial (n - 1);
}
```

$$T(n) = \begin{cases} a & n == 0 \end{cases}$$

Example 1: factorial()

```
int factorial (int n)
{
    if (n == 0)
        return 1;

    return n * factorial (n - 1);
}
```

$$T(n) = \begin{cases} a & n == 0 \end{cases}$$

Example 1: factorial()

```
int factorial (int n)
{
    if (n == 0)
        return 1;

    return n * factorial (n - 1);
}
```

$$T(n) = \begin{cases} a & n == 0 \end{cases}$$

Example 1: factorial()

```
int factorial (int n)
{
    if (n == 0)
        return 1;

    return n * factorial (n - 1);
}
```

$$T(n) = \begin{cases} a & n == 0 \\ & n > 0 \end{cases}$$

Example 1: factorial()

```
int factorial (int n)
{
    if (n == 0)
        return 1;

    return n * factorial (n - 1);
}
```

$$T(n) = \begin{cases} a & n == 0 \\ T(n-1) & n > 0 \end{cases}$$

Example 1: factorial()

```
int factorial (int n)
{
    if (n == 0)
        return 1;

    return n * factorial (n - 1);
}
```

$$T(n) = \begin{cases} a & n == 0 \\ T(n-1) + b & n > 0 \end{cases}$$

Example 1: factorial()

```
int factorial (int n)
{
    if (n == 0)
        return 1;

    return n * factorial (n - 1);
}
```

$$T(n) = \begin{cases} a & n == 0 \\ T(n-1)+b & n > 0 \end{cases}$$

Recurrence is algorithmic

A recurrence $T(n)$ is *algorithmic* if, for every sufficiently large threshold constant $n_0 > 0$, the following properties hold:

- 1 $\forall n < n_0, T(n) = \Theta(1)$
- 2 $\forall n \geq n_0$, every path of recursion terminates in a defined base case within a finite number of recursive invocations.

Convention for recurrences: *Whenever a recurrence is stated without an explicit base case, we assume that the recurrence is algorithmic.*

Example 2: displayLine()

```
void displayLine (int n)
```

```
{
```

```
    if (n > 0)
```

```
    {
```

```
        print ('=');
```

```
        displayLine (n - 1);
```

```
    }
```

```
}
```

}

Example 2: displayLine()

```
void displayLine (int n)
{
    if (n > 0)
    {
        print ('=');
        displayLine (n - 1);
    }
}
```

$$T(n) = \left\{ \right.$$

Example 2: displayLine()

```
void displayLine (int n)
```

```
{
```

```
    if (n > 0)
```

```
    {
```

```
        print ('=');
```

```
        displayLine (n - 1);
```

```
    }
```

```
}
```

$$T(n) = \left\{ \right.$$

Example 2: displayLine()

```
void displayLine (int n)
```

```
{
```

```
    if (n > 0)
```

```
    {
```

```
        print ('=');
```

```
        displayLine (n - 1);
```

```
    }
```

```
}
```

$$T(n) = \left\{ \begin{array}{l} \text{if } n > 0 \\ \text{print ('=');} \\ \text{displayLine (n - 1);} \end{array} \right.$$

$$n > 0$$

Example 2: displayLine()

```
void displayLine (int n)
```

```
{
```

```
    if (n > 0)
```

```
    {
```

```
        print ('=');
```

```
        displayLine (n - 1);
```

```
    }
```

```
}
```

$$T(n) = \begin{cases} T(n-1) & n > 0 \end{cases}$$

Example 2: displayLine()

```
void displayLine (int n)
```

```
{
```

```
    if (n > 0)
```

```
    {
```

```
        print ('=');
```

```
        displayLine (n - 1);
```

```
    }
```

```
}
```

$$T(n) = \begin{cases} T(n-1) + b & n > 0 \end{cases}$$

Example 2: displayLine()

```
void displayLine (int n)
{
    if (n > 0)
    {
        print ('=');
        displayLine (n - 1);
    }
}
```

$$T(n) = \begin{cases} n == 0 & \\ T(n-1)+b & n > 0 \end{cases}$$

Example 2: displayLine()

```
void displayLine (int n)
{
    if (n > 0)
    {
        print ('=');
        displayLine (n - 1);
    }
}
```

$$T(n) = \begin{cases} a & n == 0 \\ T(n-1) + b & n > 0 \end{cases}$$

Example 2: displayLine()

```
void displayLine (int n)
{
    if (n > 0)
    {
        print ('=');
        displayLine (n - 1);
    }
}
```

$$T(n) = \begin{cases} a & n == 0 \\ T(n-1) + b & n > 0 \end{cases}$$

Exercise 1

Write the recursive function and derive its recurrence relation.

- ① `sum (n)` : computes for $\sum_{j=1}^n j$
- ② `power (x, y)` : computes for x^y
- ③ `fibonacci (n)` : returns the n^{th} fibonacci number.

Fibonacci numbers are: 0, 1, 1, 2, 3, 5, 8, 13, 21, ...

Solving recurrences: Iteration Method

Determine the closed form or explicit formula of $T(n)$.

Solving recurrences: Iteration Method

Determine the closed form or explicit formula of $T(n)$.

$$T(n) = \begin{cases} 2 & n = 1 \\ T(n-1) + 3 & n > 1 \end{cases}$$

Solving recurrences: Iteration Method

Determine the closed form or explicit formula of $T(n)$.

$$T(n) = \begin{cases} 2 & n = 1 \\ T(n-1) + 3 & n > 1 \end{cases}$$

set $n = 5$,

Solving recurrences: Iteration Method

Determine the closed form or explicit formula of $T(n)$.

$$T(n) = \begin{cases} 2 & n = 1 \\ T(n-1) + 3 & n > 1 \end{cases}$$

set $n = 5$,

$$T(5)$$

Solving recurrences: Iteration Method

Determine the closed form or explicit formula of $T(n)$.

$$T(n) = \begin{cases} 2 & n = 1 \\ T(n-1) + 3 & n > 1 \end{cases}$$

set $n = 5$,

$$T(5) = T(5) \quad (1)$$

Solving recurrences: Iteration Method

Determine the closed form or explicit formula of $T(n)$.

$$T(n) = \begin{cases} 2 & n = 1 \\ T(n-1) + 3 & n > 1 \end{cases}$$

set $n = 5$,

$$T(5) = T(4) + 3 \quad (1)$$

Solving recurrences: Iteration Method

Determine the closed form or explicit formula of $T(n)$.

$$T(n) = \begin{cases} 2 & n = 1 \\ T(n-1) + 3 & n > 1 \end{cases}$$

set $n = 5$,

$$T(5) = T(4) + 3 \quad (1)$$

$$= T(4) + 3 \quad (2)$$

Solving recurrences: Iteration Method

Determine the closed form or explicit formula of $T(n)$.

$$T(n) = \begin{cases} 2 & n = 1 \\ T(n-1) + 3 & n > 1 \end{cases}$$

set $n = 5$,

$$T(5) = T(4) + 3 \quad (1)$$

$$= T(3) + 3 + 3 \quad (2)$$

Solving recurrences: Iteration Method

Determine the closed form or explicit formula of $T(n)$.

$$T(n) = \begin{cases} 2 & n = 1 \\ T(n-1) + 3 & n > 1 \end{cases}$$

set $n = 5$,

$$T(5) = T(4) + 3 \quad (1)$$

$$= T(3) + 3 + 3 \quad (2)$$

$$= T(3) + 3 + 3 \quad (3)$$

Solving recurrences: Iteration Method

Determine the closed form or explicit formula of $T(n)$.

$$T(n) = \begin{cases} 2 & n = 1 \\ T(n-1) + 3 & n > 1 \end{cases}$$

set $n = 5$,

$$T(5) = T(4) + 3 \quad (1)$$

$$= T(3) + 3 + 3 \quad (2)$$

$$= T(2) + 3 + 3 + 3 \quad (3)$$

Solving recurrences: Iteration Method

Determine the closed form or explicit formula of $T(n)$.

$$T(n) = \begin{cases} 2 & n = 1 \\ T(n-1) + 3 & n > 1 \end{cases}$$

set $n = 5$,

$$T(5) = T(4) + 3 \quad (1)$$

$$= T(3) + 3 + 3 \quad (2)$$

$$= T(2) + 3 + 3 + 3 \quad (3)$$

$$= T(2) + 3 + 3 + 3 \quad (4)$$

Solving recurrences: Iteration Method

Determine the closed form or explicit formula of $T(n)$.

$$T(n) = \begin{cases} 2 & n = 1 \\ T(n-1) + 3 & n > 1 \end{cases}$$

set $n = 5$,

$$T(5) = T(4) + 3 \quad (1)$$

$$= T(3) + 3 + 3 \quad (2)$$

$$= T(2) + 3 + 3 + 3 \quad (3)$$

$$= T(1) + 3 + 3 + 3 + 3 \quad (4)$$

Solving recurrences: Iteration Method

Determine the closed form or explicit formula of $T(n)$.

$$T(n) = \begin{cases} 2 & n = 1 \\ T(n-1) + 3 & n > 1 \end{cases}$$

set $n = 5$,

$$T(5) = T(4) + 3 \quad (1)$$

$$= T(3) + 3 + 3 \quad (2)$$

$$= T(2) + 3 + 3 + 3 \quad (3)$$

$$= T(1) + 3 + 3 + 3 + 3 \quad (4)$$

$$= T(1) + 3 + 3 + 3 + 3 \quad (5)$$

Solving recurrences: Iteration Method

Determine the closed form or explicit formula of $T(n)$.

$$T(n) = \begin{cases} 2 & n = 1 \\ T(n-1) + 3 & n > 1 \end{cases}$$

set $n = 5$,

$$T(5) = T(4) + 3 \quad (1)$$

$$= T(3) + 3 + 3 \quad (2)$$

$$= T(2) + 3 + 3 + 3 \quad (3)$$

$$= T(1) + 3 + 3 + 3 + 3 \quad (4)$$

$$= 2 + 3 + 3 + 3 + 3 \quad (5)$$

Solving recurrences: Iteration Method

Determine the closed form or explicit formula of $T(n)$.

$$T(n) = \begin{cases} 2 & n = 1 \\ T(n-1) + 3 & n > 1 \end{cases}$$

set $n = 5$,

$$T(5) = T(4) + 3 \quad (1)$$

$$= T(3) + 3 + 3 \quad (2)$$

$$= T(2) + 3 + 3 + 3 \quad (3)$$

$$= T(1) + 3 + 3 + 3 + 3 \quad (4)$$

$$= 2 + 3 + 3 + 3 + 3 \quad (5)$$

$$T(5) = 2 + 3(4) \quad (6)$$

Solving recurrences: Iteration Method

Determine the closed form or explicit formula of $T(n)$.

$$T(n) = \begin{cases} 2 & n = 1 \\ T(n-1) + 3 & n > 1 \end{cases}$$

set $n = 5$,

$$T(5) = T(4) + 3 \quad (1)$$

$$= T(3) + 3 + 3 \quad (2)$$

$$= T(2) + 3 + 3 + 3 \quad (3)$$

$$= T(1) + 3 + 3 + 3 + 3 \quad (4)$$

$$= 2 + 3 + 3 + 3 + 3 \quad (5)$$

$$T(5) = 2 + 3(4) \quad (6)$$

If $n = 5$, $__ = 4$.

Solving recurrences: Iteration Method

Determine the closed form or explicit formula of $T(n)$.

$$T(n) = \begin{cases} 2 & n = 1 \\ T(n-1) + 3 & n > 1 \end{cases}$$

set $n = 5$,

$$T(5) = T(4) + 3 \quad (1)$$

$$= T(3) + 3 + 3 \quad (2)$$

$$= T(2) + 3 + 3 + 3 \quad (3)$$

$$= T(1) + 3 + 3 + 3 + 3 \quad (4)$$

$$= 2 + 3 + 3 + 3 + 3 \quad (5)$$

$$T(5) = 2 + 3(4) \quad (6)$$

If $n = 5$, $__ = 4$.

$$T(5) = 2 + 3(4) \quad (7)$$

Solving recurrences: Iteration Method

Determine the closed form or explicit formula of $T(n)$.

$$T(n) = \begin{cases} 2 & n = 1 \\ T(n-1) + 3 & n > 1 \end{cases}$$

set $n = 5$,

$$T(5) = T(4) + 3 \quad (1)$$

$$= T(3) + 3 + 3 \quad (2)$$

$$= T(2) + 3 + 3 + 3 \quad (3)$$

$$= T(1) + 3 + 3 + 3 + 3 \quad (4)$$

$$= 2 + 3 + 3 + 3 + 3 \quad (5)$$

$$T(5) = 2 + 3(4) \quad (6)$$

$$T(n) = 2 + 3(n-1) \quad (7)$$

Solving recurrences: Iteration Method

Determine the closed form or explicit formula of $T(n)$.

$$T(n) = \begin{cases} 2 & n = 1 \\ T(n-1) + 3 & n > 1 \end{cases}$$

set $n = 5$,

$$T(5) = T(4) + 3 \quad (1)$$

$$= T(3) + 3 + 3 \quad (2)$$

$$= T(2) + 3 + 3 + 3 \quad (3)$$

$$= T(1) + 3 + 3 + 3 + 3 \quad (4)$$

$$= 2 + 3 + 3 + 3 + 3 \quad (5)$$

$$T(5) = 2 + 3(4) \quad (6)$$

$$T(n) = 2 + 3(n-1) \quad (7) \quad \text{Simplify!}$$

Solving recurrences: Iteration Method

Determine the closed form or explicit formula of $T(n)$.

$$T(n) = \begin{cases} 2 & n = 1 \\ T(n-1) + 3 & n > 1 \end{cases}$$

set $n = 5$,

$$T(5) = T(4) + 3 \quad (1)$$

$$= T(3) + 3 + 3 \quad (2)$$

$$= T(2) + 3 + 3 + 3 \quad (3)$$

$$= T(1) + 3 + 3 + 3 + 3 \quad (4)$$

$$= 2 + 3 + 3 + 3 + 3 \quad (5)$$

$$T(5) = 2 + 3(4) \quad (6)$$

$$T(n) = 2 + 3(n-1) \quad (7) \quad \text{Simplify!}$$

$$= 2 + 3n - 3 \quad (8)$$

Solving recurrences: Iteration Method

Determine the closed form or explicit formula of $T(n)$.

$$T(n) = \begin{cases} 2 & n = 1 \\ T(n-1) + 3 & n > 1 \end{cases}$$

set $n = 5$,

$$T(5) = T(4) + 3 \quad (1)$$

$$= T(3) + 3 + 3 \quad (2)$$

$$= T(2) + 3 + 3 + 3 \quad (3)$$

$$= T(1) + 3 + 3 + 3 + 3 \quad (4)$$

$$= 2 + 3 + 3 + 3 + 3 \quad (5)$$

$$T(5) = 2 + 3(4) \quad (6)$$

$$T(n) = 2 + 3(n-1) \quad (7)$$

$$= 2 + 3n - 3 \quad (8)$$

$$= 3n - 1 \quad (9)$$

Simplify!

Solving recurrences: Iteration Method

Determine the closed form or explicit formula of $T(n)$.

$$T(n) = \begin{cases} 2 & n = 1 \\ T(n-1) + 3 & n > 1 \end{cases}$$

set $n = 5$,

$$T(5) = T(4) + 3 \quad (1)$$

$$= T(3) + 3 + 3 \quad (2)$$

$$= T(2) + 3 + 3 + 3 \quad (3)$$

$$= T(1) + 3 + 3 + 3 + 3 \quad (4)$$

$$= 2 + 3 + 3 + 3 + 3 \quad (5)$$

$$T(5) = 2 + 3(4) \quad (6)$$

$$T(n) = 2 + 3(n-1) \quad (7)$$

$$= 2 + 3n - 3 \quad (8)$$

$$T(n) = 3n - 1 \quad (9)$$

Solving recurrences: Iteration Method

Determine the closed form or explicit formula of $T(n)$.

$$T(n) = \begin{cases} 2 & n = 1 \\ T(n-1) + 3 & n > 1 \end{cases}$$

set $n = 5$,

$$T(5) = T(4) + 3 \quad (1)$$

$$= T(3) + 3 + 3 \quad (2)$$

$$= T(2) + 3 + 3 + 3 \quad (3)$$

$$= T(1) + 3 + 3 + 3 + 3 \quad (4)$$

$$= 2 + 3 + 3 + 3 + 3 \quad (5)$$

$$T(5) = 2 + 3(4) \quad (6)$$

$$T(n) = 2 + 3(n-1) \quad (7)$$

$$= 2 + 3n - 3 \quad (8)$$

$$T(n) = 3n - 1 \quad O(n) \quad (9)$$

Exercise 2

Use the iteration method to determine the explicit formula and the *Big-Oh* of the following recurrences defined.

$$① \quad T(n) = \begin{cases} a & n = 1 \\ T(n-1) + b & n > 1 \end{cases}$$

$$② \quad T(n) = \begin{cases} 5 & n = 0 \\ T(n-1) + 2n - 1 & n > 0 \end{cases}$$

$$③ \quad T(n) = \begin{cases} 1 & n = 1 \\ T\left(\frac{n}{2}\right) + 1 & n > 1 \end{cases}$$

$$④ \quad T(n) = \begin{cases} 8 & n = 1 \\ 2T(n-1) + 5 & n > 1 \end{cases}$$

$$⑤ \quad T(n) = \begin{cases} 1 & n = 1 \\ 2T\left(\frac{n}{2}\right) + 1 & n > 1 \end{cases}$$

Formulas to **recall** : Summations

$$\sum_{j=a}^b 1 = b - a + 1$$

$$\sum_{j=0}^n j = \frac{n(n+1)}{2}$$

$$\sum_{j=0}^n j^2 = \frac{n(n+1)(2n+1)}{6}$$

$$\sum_{j=0}^n j^3 = \frac{n^2(n+1)^2}{4}$$

$$\sum_{j=0}^n x^j = \frac{x^{n+1} - 1}{x - 1}$$

Logarithms

Notations:

$\lg n = \log_2 n$ binary logarithm

$\ln n = \log_e n$ natural logarithm

$\lg^k n = (\lg n)^k$ exponentiation

$\lg \lg n = \lg(\lg n)$ composition

$\log n + 1 = (\log n) + 1 \neq \log(n + 1)$

For any constant $b > 1$,

$$\log_b n = \begin{cases} \text{undefined} & n \leq 0 \\ \text{strictly increasing} & n > 0 \\ \text{negative} & 0 < n < 1 \\ \text{positive} & n > 1 \\ 0 & n = 1 \end{cases}$$

Formulas to remember : Logarithms

For all real $a > 0, b > 0, c > 0, n$, and logarithm bases $\neq 1$

$$a = b^{\log_b a}$$

$$\log_c ab = \log_c a + \log_c b$$

$$\log_b a^n = n \log_b a$$

$$\log_b \frac{1}{a} = -\log_b a$$

$$\log_b a = \frac{\log_c a}{\log_c b}$$

$$\log_b a = \frac{1}{\log_a b}$$

$$a^{\log_b c} = c^{\log_b a}$$

Reference

Antioquia, A. (2020). Recurrences. CCDSALG Lecture.

Cormen, T., Leiserson, C., Rivest, R., and Stein, C. (2022). Introduction to Algorithms, fourth edition. MIT Press.